Dom.lean
@@ -94,6 +94,8 @@ import Dom.Spec.Move
 import Dom.Spec.MoveSound
 import Dom.Spec.MoveCongr
 import Dom.Spec.Complete
+import Dom.Spec.PreInsertValidity
+import Dom.Properties.PreInsertValidityBridge
 import Dom.Spec.Result
 import Dom.Properties.Counterexample
 import Dom.Properties.Witness
